progs/verif_cond.v
@@ -151,13 +151,13 @@ Lemma prog_correct:
   semax_prog prog Vprog Gprog.
 Proof.
 prove_semax_prog.
-repeat (apply semax_func_cons_ext_vacuous; [reflexivity | reflexivity | ]).
+repeat (apply semax_func_cons_ext_vacuous; [reflexivity | reflexivity| reflexivity | reflexivity]).
+semax_func_cons_ext.
+semax_func_cons_ext. 
 semax_func_cons_ext.
 semax_func_cons_ext.
 semax_func_cons_ext.
-semax_func_cons_ext.
-semax_func_cons_ext.
-semax_func_cons_ext.
+semax_func_cons_ext. 
 semax_func_cons_ext.
 semax_func_cons_ext.
 semax_func_cons_ext.
@@ -165,4 +165,4 @@ semax_func_cons_ext.
 semax_func_cons_ext.
 semax_func_cons body_thread_func.
 semax_func_cons body_main.
-Qed.
+Admitted. (*Proof complete, but Qed does not terminate*)
